experiment/Experiment.Steel.Combinators.Tac.fst
@@ -1,0 +1,277 @@
+module Experiment.Steel.Combinators.Tac
+
+include Experiment.Steel.Combinators
+
+module U  = Learn.Util
+module L  = FStar.List.Pure
+module SH = Experiment.Steel.Steel
+
+open FStar.Tactics
+open Learn.Tactics.Util
+open Experiment.Steel.Interface
+open Experiment.Steel.Repr.M
+open Experiment.Steel.Tac
+
+
+(*** Lifts *)
+
+(***** [erasable_t] *)
+
+private unfold
+let __build_revealed_value (a : Type) : (x : Ghost.erased a) -> GTot (revealed_value x)
+  = fun x -> Ghost.reveal x
+
+/// Solves a goal [erasable_t a] if a is an erasable type.
+let build_erasable_t fr ctx : Tac unit
+  =
+    let a : term
+      = match inspect (cur_goal ()) with
+        | Tv_App  _ arg -> arg._1
+        | _ -> fail "build_erasable_t : goal"
+    in
+    apply (`Mkerasable_t);
+    // The following requires a conversion from [_ -> GTot (revealed_value x)] to [_ -> Tot (revealed_value x)]
+    // which succeeds iff [revealed_value x] (i.e. [a]) is erasable.
+    // Since we use (`#a), this may generate some guards to retypecheck (`#a).
+    with_policy SMT (fun () -> cs_try (fun () ->
+      exact (`(__build_revealed_value (`#a) <: _ -> Tot _)))
+    fr ctx (fun m -> fail (m (Fail_not_erasable a) [])))
+
+private
+let test_erasable_unit : erasable_t unit
+  = _ by (build_erasable_t default_flags dummy_ctx)
+
+private
+let test_erasable_unit' : erasable_t U.unit'
+  = _ by (build_erasable_t default_flags dummy_ctx)
+
+#push-options "--silent"
+[@@ expect_failure [228]]
+private
+let test_erasable_int : erasable_t int
+  = _ by (build_erasable_t default_flags dummy_ctx)
+#pop-options
+
+[@@ erasable]
+private noeq
+type test_guard_type (_ : squash (forall (n : nat) . n >= 0)) =
+
+private
+let test_erasable_guard : erasable_t (test_guard_type ())
+  = _ by (build_erasable_t default_flags dummy_ctx)
+
+
+(***** [steel_liftable] *)
+
+
+/// Solves a goal [C.steel_liftable a ek0 ek1].
+/// Since we start by trying to apply [C.Rt1n_refl], if [ek0] or [ek1] is an uvar, we will choose a trivial lift.
+let rec build_steel_liftable_aux fr ctx : Tac unit
+  =
+    try apply (`Rt1n_refl)
+    with _ ->
+      apply (`Rt1n_trans);
+      // lift1
+      begin
+        match catch (fun () -> apply (`Lift_ghost_ghostI)) with
+        | Inr () -> build_erasable_t fr ctx
+        | Inl _ ->
+        try apply (`Lift_ghostI_atomic) with _ ->
+        try apply (`Lift_atomic_steel)  with _ ->
+        cs_raise fr ctx (fun m -> fail (m Fail_liftable []))
+      end;
+
+      build_steel_liftable_aux fr ctx
+
+let build_steel_liftable fr ctx : Tac unit
+  =
+    let goal = cur_goal () in
+    build_steel_liftable_aux fr (ctx_app_info ctx [Info_goal goal])
+
+
+(*** Combinable *)
+
+(***** [effect_kind_enum] *)
+
+type effect_kind_enum = | ESteel | EAtomic | EGhostI | EGhost
+
+let ek_ord (ek : effect_kind_enum) : int
+  = match ek with
+  | EGhost  -> 0
+  | EGhostI -> 1
+  | EAtomic -> 2
+  | ESteel  -> 3
+
+let ek_le (ek0 ek1 : effect_kind_enum) : bool
+  = ek_ord ek0 <= ek_ord ek1
+
+/// Given a term representing a [SH.effect_kind], returns the corresponding [effect_kind_enum].
+let collect_effect_kind fr ctx (t : term) : Tac (option effect_kind_enum)
+  =
+    if Tv_Uvar? (inspect t) then None
+    else begin
+      let hd = cs_try (fun () -> collect_fvar (collect_app t)._1)
+                 fr ctx (fun m -> fail (m (Fail_goal_shape GShape_effect_kind) [])) in
+      Some (if hd = (`%SH.KSteel ) then ESteel
+       else if hd = (`%SH.KAtomic) then EAtomic
+       else if hd = (`%SH.KGhostI) then EGhostI
+       else if hd = (`%SH.KGhost ) then EGhost
+       else cs_raise fr ctx (fun m -> fail (m (Fail_goal_shape GShape_effect_kind) [])))
+    end
+
+/// Used to mark the definitions that have to be unfolded before collecting an [effect_kind].
+irreducible let __effect_kind__ : unit = ()
+
+
+(***** bind *)
+
+[@@ __extraction__]
+noeq inline_for_extraction
+type bind_combinable (a0 a1 : Type u#a) (ek0 ek1 ek2 : SH.effect_kind) = {
+  cba_bind_ek0'  : SH.effect_kind;
+  cba_bind_ek1'  : SH.effect_kind;
+  cba_bind_ek2'  : SH.effect_kind;
+  cba_bind_steel : bind_steel_t u#a u#p cba_bind_ek0' cba_bind_ek1' cba_bind_ek2';
+  cba_bind_lift0 : steel_liftable a0 ek0 cba_bind_ek0';
+  cba_bind_lift1 : steel_liftable a1 ek1 cba_bind_ek1';
+  cba_bind_lift2 : steel_liftable a1 cba_bind_ek2' ek2;
+}
+
+[@@ __repr_M__]
+let bind_combinable_repr
+      #a0 #a1 #ek0 #ek1 #ek2 (c : bind_combinable u#a u#p a0 a1 ek0 ek1 ek2)
+      (f : repr ek0 a0) (g : a0 -> repr ek1 a1)
+  : repr ek2 a1
+  =
+    let f' = repr_lift c.cba_bind_lift0 f              in
+    let g' (x : a0) = repr_lift c.cba_bind_lift1 (g x) in
+    let r' = bind_ek _ _ _ c.cba_bind_steel f' g'      in
+    repr_lift c.cba_bind_lift2 r'
+
+let bind_steel_t_for (ek0 ek1 : effect_kind_enum) : term
+  = match if ek0 `ek_le` ek1 then ek1 else ek0 with
+  | EGhost  -> (`bind_steel__ghost)
+  | EGhostI -> (`bind_steel__ghostI)
+  | EAtomic -> let ek' = if ek0 `ek_le` ek1 then ek1 else ek0 in
+              if ek' `ek_le` EGhostI
+              then (if ek0 = EAtomic then (`bind_steel__atomic_ghost) else (`bind_steel__ghost_atomic))
+              else (`bind_steel__steel)
+  | ESteel  -> (`bind_steel__steel)
+
+/// Solves a goal [bind_combinable a0 a1 ek0' ek1' ek2'] where [ek0], [ek1] should match [ek0'], [ek1'].
+let build_bind_combinable fr ctx ek0 ek1 : Tac unit
+  =
+    let op = bind_steel_t_for ek0 ek1 in
+    apply (`Mkbind_combinable);
+    // cba_bind_repr
+    seq (fun () -> apply op) dismiss;
+    // cba_bind_lift0
+    build_steel_liftable fr ctx;
+    // cba_bind_lift1
+    build_steel_liftable fr ctx;
+    // cba_bind_lift2
+    build_steel_liftable fr ctx
+
+
+(***** if-then-else *)
+
+[@@ __extraction__]
+noeq
+type ite_combinable (a : Type u#a) (ek0 ek1 ek2 : SH.effect_kind) = {
+  cba_ite_ek2'  : cba_ite_effect_kind_t;
+  cba_ite_lift0 : steel_liftable a ek0 cba_ite_ek2';
+  cba_ite_lift1 : steel_liftable a ek1 cba_ite_ek2';
+  cba_ite_lift2 : steel_liftable a cba_ite_ek2' ek2;
+}
+
+
+[@@ __effect_kind__] let combinable_ite_ghost  o : cba_ite_effect_kind_t =  SH.KGhost  o
+[@@ __effect_kind__] let combinable_ite_ghostI o : cba_ite_effect_kind_t = (SH.KGhostI o)
+[@@ __effect_kind__] let combinable_ite_steel    : cba_ite_effect_kind_t =  SH.KSteel
+
+let combinable_ite_kind (ek0 ek1 : effect_kind_enum) : term
+  = match if ek0 `ek_le` ek1 then ek1 else ek0 with
+  | EGhost  -> (`combinable_ite_ghost)
+  | EGhostI -> (`combinable_ite_ghostI)
+  | EAtomic | ESteel -> (`combinable_ite_steel)
+
+/// Solves a goal [ite_combinable a ek0' ek1' ek2'] where [ek0], [ek1] should match [ek0'], [ek1'].
+let build_ite_combinable fr ctx ek0 ek1 : Tac unit
+  =
+    let ek = combinable_ite_kind ek0 ek1 in
+    apply_raw (`Mkite_combinable);
+    // cba_ite_ek2'
+    seq (fun () -> apply ek) dismiss;
+    // cba_ite_lift0
+    build_steel_liftable fr ctx;
+    // cba_ite_lift1
+    build_steel_liftable fr ctx;
+    // cba_ite_lift2
+    build_steel_liftable fr ctx
+
+
+(*** [solve_combinables] *)
+
+/// [solve_combinables] should be called on a state where all goals are of one of the form:
+/// - [steel_liftable a ek1 ek2]
+/// - [combinable_bind_t a0 a1 ek0 ek1 ek2]
+/// - [combinable_ite_t a ek0 ek1 ek2]
+/// It tries to solve them. It fails if it reaches a state where it cannot make progress on any goal.
+
+/// Try to solves a goal.
+/// - succeed and returns true if the heads of ek0 and ek1 are known.
+/// - otherwise, returns false.
+let build_combinable fr ctx : Tac bool
+  =
+    // there are some beta-redexes + aliases
+    norm [delta_attr [`%__effect_kind__]];
+    
+    let hd, args = collect_app (cur_goal ()) in
+    let hd = try collect_fvar hd with _ -> "unexpected shape" in
+    if hd = (`%steel_liftable)
+    then begin
+      guard (L.length args = 3);
+      let ek1 = collect_effect_kind fr ctx (L.index args 1)._1 in
+      match ek1 with
+      | Some _ -> build_steel_liftable fr ctx; true
+      | _ -> false
+    end else if hd = (`%bind_combinable)
+    then begin
+      guard (L.length args = 5);
+      let ek0 = collect_effect_kind fr ctx (L.index args 2)._1 in
+      let ek1 = collect_effect_kind fr ctx (L.index args 3)._1 in
+      match ek0, ek1 with
+      | Some ek0, Some ek1 -> build_bind_combinable fr ctx ek0 ek1; true
+      | _ -> false
+    end else if hd = (`%ite_combinable)
+    then begin
+      guard (L.length args = 4);
+      let ek0 = collect_effect_kind fr ctx (L.index args 1)._1 in
+      let ek1 = collect_effect_kind fr ctx (L.index args 2)._1 in
+      match ek0, ek1 with
+      | Some ek0, Some ek1 -> build_ite_combinable fr ctx ek0 ek1; true
+      | _ -> false
+    end else fail "build_combinable : goal_shape"
+
+let rec solve_combinables_round fr : Tac (bool & list goal)
+  = match goals () with
+    | [] -> false, []
+    | g :: _ ->
+        if build_combinable fr dummy_ctx
+        then
+          let _, gs = solve_combinables_round fr in
+          true, gs
+        else begin
+          dismiss ();
+          let b, gs = solve_combinables_round fr in
+          b, g :: gs
+        end
+
+let rec solve_combinables fr : Tac unit
+  = match goals () with
+  | [] -> ()
+  | _ :: _ ->
+    let b, gs = solve_combinables_round fr in
+    if not b then cs_raise fr dummy_ctx (fun m -> fail (m Fail_solve_combinables []));
+    set_goals gs;
+    solve_combinables fr
