experiment/Experiment.Steel.Monad.fst
@@ -3,7 +3,7 @@ module Experiment.Steel.Monad
 include Experiment.Steel.Interface
 
 module M   = Experiment.Steel.Repr.M
-module MC  = Experiment.Steel.Combinators
+module C   = Experiment.Steel.Combinators.Tac
 module SE  = Steel.Effect
 module SA  = Steel.Effect.Atomic
 module SH  = Experiment.Steel.Steel
@@ -11,6 +11,102 @@ module Mem = Steel.Memory
 
 open FStar.Tactics
 open Experiment.Steel
+
+
+irreducible let __monad_implicit__ : unit = ()
+
+[@@ __repr_M__]
+let return_hint (#a : Type) (#opened: Mem.inames) (x : a) (sl_hint : M.post_t a)
+  : M.repr (SH.KGhostI opened) a
+  = C.return_hint (SH.KGhostI opened) #a x (Some sl_hint)
+
+[@@ __repr_M__]
+let return (#a : Type) (#opened: Mem.inames) (x : a)
+  : M.repr (SH.KGhostI opened) a
+  = C.return (SH.KGhostI opened) #a x
+
+[@@ __repr_M__]
+let return_hint_g (#a : Type) (#opened: Mem.inames) (x : a) (sl_hint : M.post_t a)
+  : M.repr (SH.KGhost opened) a
+  = C.return_hint (SH.KGhost opened) #a x (Some sl_hint)
+
+[@@ __repr_M__]
+let return_g (#a : Type) (#opened: Mem.inames) (x : a)
+  : M.repr (SH.KGhost opened) a
+  = C.return (SH.KGhost opened) #a x
+
+[@@ __repr_M__]
+let bind
+      (#a #b : Type u#a)
+      (#ek0 #ek1 #ek2 : SH.effect_kind)
+      (#[@@@ __monad_implicit__] cba : C.bind_combinable u#a u#p a b ek0 ek1 ek2)
+      (f : M.repr ek0 a) (g : a -> M.repr ek1 b)
+  : M.repr ek2 b
+  = C.bind_combinable_repr cba f g
+
+[@@ __repr_M__]
+let ite
+      (#a : Type) (guard : bool)
+      (#ek0 #ek1 #ek2 : SH.effect_kind) 
+      (#[@@@ __monad_implicit__] cba : C.ite_combinable a ek0 ek1 ek2)
+      (thn : M.repr ek0 a) (els : M.repr ek1 a)
+  : M.repr ek2 a
+  = C.repr_lift cba.cba_ite_lift2
+      (C.ite cba.cba_ite_ek2' guard
+        (C.repr_lift cba.cba_ite_lift0 thn)
+        (C.repr_lift cba.cba_ite_lift1 els))
+
+
+/// Calling a Steel function from our representation
+[@@ __repr_M__]
+let call (#b : Type)
+      (#a : b -> Type) (#pre : b -> SE.pre_t) (#post : (x : b) -> SE.post_t (a x))
+      (#req : (x : b) -> SE.req_t (pre x)) (#ens : (x : b) -> SE.ens_t (pre x) (a x) (post x))
+      ($f : (x : b) -> SE.Steel (a x) (pre x) (post x) (req x) (ens x)) (x : b)
+  : M.repr SH.KSteel (a x)
+  = C.repr_of_steel (pre x) (post x) (req x) (ens x) (SH.steel_fe (fun () -> f x))
+
+[@@ __repr_M__]
+let call_g (#b : Type)
+      (#a : b -> Type) (#opened : b -> Mem.inames) (#pre : b -> SE.pre_t) (#post : (x : b) -> SE.post_t (a x))
+      (#req : (x : b) -> SE.req_t (pre x)) (#ens : (x : b) -> SE.ens_t (pre x) (a x) (post x))
+      ($f : (x : b) -> SA.SteelGhost (a x) (opened x) (pre x) (post x) (req x) (ens x)) (x : b)
+  : M.repr (SH.KGhost (opened x)) (a x)
+  = C.repr_of_steel (pre x) (post x) (req x) (ens x) (SH.ghost_fe (fun () -> f x))
+
+let __assert_sq (#opened : Mem.inames) (p : Type)
+  : SA.SteelGhost (squash p) opened SA.emp (fun _ -> SA.emp) (requires fun _ -> p) (ensures fun _ _ _ -> True)
+  = SA.noop ()
+
+[@@ __repr_M__]
+let assert_sq (#opened : Mem.inames) (p : Type)
+  : M.repr (SH.KGhost opened) (squash p)
+  = call_g __assert_sq p // TODO use a spec_r_exact
+
+/// Does not work because it requires to recheck the monotonicity of wp.
+[@@ __repr_M__]
+let pure (#a : Type) (#wp : pure_wp a) ($f : unit -> PURE a wp)
+  : M.repr SH.KSteel a
+  = C.bindP SH.KSteel wp f (fun x -> C.return SH.KSteel x)
+
+let __ghost (#a : Type) (#opened : Mem.inames) (x : Ghost.erased a)
+  : SA.SteelGhost a opened SA.emp (fun _ -> SA.emp) (fun _ -> True) (fun _ _ _ -> True)
+  = SA.noop (); x
+
+[@@ __repr_M__]
+let ghost (#a : Type) (#opened : Mem.inames) (x : Ghost.erased a)
+  : M.repr (SH.KGhost opened) a
+  = call_g __ghost x // TODO use a spec_r_exact
+
+/// Used when a combinator expect a specific effect. An alternative would be a bind with [noop] but this lift does
+/// not change the [repr_tree].
+[@@ __repr_M__]
+let elift
+      (#a : Type)
+      (#ek0 #ek1 : SH.effect_kind) (#[@@@ __monad_implicit__] lt : C.steel_liftable a ek0 ek1)
+      (f : M.repr ek0 a)
+  : M.repr ek1 a
+  = C.repr_lift lt f
 
 
 unfold
@@ -27,52 +123,16 @@ let mk_steel (fs : list flag) : Tac unit
 unfold
 let to_steel
       (#a : Type) (#pre : SE.pre_t) (#post : SE.post_t a) (#req : SE.req_t pre) (#ens : SE.ens_t pre a post)
-      (t : M.repr SH.KSteel a)
-      (#[exact (`(_ by (mk_steel [])))] g : __to_steel_goal a pre post req ens t) ()
+      (#ek0 : SH.effect_kind) (#[@@@ __monad_implicit__] lt : C.steel_liftable a ek0 SH.KSteel)
+      (t : M.repr ek0 a)
+      (#[exact (`(_ by (mk_steel [])))] g : __to_steel_goal a pre post req ens (C.repr_lift lt t)) ()
   : steel a pre post req ens
-  = to_steel #a #pre #post #req #ens t g
+  = g
+// TODO: other effects
 
 
-unfold
-let return_hint (#a : Type) (x : a) (sl_hint : M.post_t a)
-  : M.repr SH.KSteel a
-  = MC.return_hint SH.KSteel #a x (Some sl_hint)
-
-unfold
-let return (#a : Type) (x : a)
-  : M.repr SH.KSteel a
-  = MC.return SH.KSteel #a x
-
-// TODO? generalize with typeclass
-unfold
-let bind (#a #b : Type) (f : M.repr SH.KSteel a) (g : a -> M.repr SH.KSteel b)
-  : M.repr SH.KSteel b
-  = MC.bind #a #b f g
-
-unfold
-let pure (#a : Type) (#wp : pure_wp a) ($f : unit -> PURE a wp)
-  : M.repr SH.KSteel a
-  = MC.bindP SH.KSteel wp f (fun x -> MC.return SH.KSteel x)
-
-unfold
-let ite (#a : Type) (guard : bool) (thn : M.repr SH.KSteel a) (els : M.repr SH.KSteel a)
-  : M.repr SH.KSteel a
-  = MC.ite guard thn els
-
-
-/// Calling a Steel function from our representation
-unfold
-let call (#b : Type)
-      (#a : b -> Type) (#pre : b -> SE.pre_t) (#post : (x : b) -> SE.post_t (a x))
-      (#req : (x : b) -> SE.req_t (pre x)) (#ens : (x : b) -> SE.ens_t (pre x) (a x) (post x))
-      ($f : (x : b) -> SE.Steel (a x) (pre x) (post x) (req x) (ens x)) (x : b)
-  : M.repr SH.KSteel (a x)
-  = MC.repr_of_steel (pre x) (post x) (req x) (ens x) (SH.steel_fe (fun () -> f x))
-
-unfold
-let call_g (#b : Type)
-      (#a : b -> Type) (#opened : b -> Mem.inames) (#pre : b -> SE.pre_t) (#post : (x : b) -> SE.post_t (a x))
-      (#req : (x : b) -> SE.req_t (pre x)) (#ens : (x : b) -> SE.ens_t (pre x) (a x) (post x))
-      ($f : (x : b) -> SA.SteelGhost (a x) (opened x) (pre x) (post x) (req x) (ens x)) (x : b)
-  : M.repr (SH.KGhost (opened x)) (a x)
-  = MC.repr_of_steel (pre x) (post x) (req x) (ens x) (SH.ghost_fe (fun () -> f x))
+[@@ resolve_implicits; __monad_implicit__]
+let monad_implicits_tac () : Tac unit
+  =
+    let fr = default_flags in
+    C.solve_combinables fr
